coq/theories/Examples/IPv4.v
@@ -1,0 +1,24 @@
+Require Import MiniP4.Syntax.
+
+Open Scope string_scope.
+
+Definition meta_t : typ :=
+  (* drop flag, port number *)
+  Prod [Bool; Bit 8].
+
+Definition ipv4_t : typ :=
+  (* src addr, dst addr *)
+  Prod [Bit 8; Bit 8].
+
+Definition zeros (n: nat) : exp :=
+  Bits (List.repeat false n).
+
+Definition ipv4_defns : list defn :=
+  [VarDecl ipv4_t "ip" (Tuple [zeros 8; zeros 8]);
+  Action "set_out" (Assign "meta" (Tuple [EBool false; zeros 8]));
+  Table "route" (Proj (Var "ip") 1) ["set_out"] ].
+
+Definition ipv4_cmd : cmd :=
+  Block [Extr "ip";
+         Apply "route";
+         Emit "ip"].
